riscV/RelocBinDecode.v
@@ -1,0 +1,35 @@
+Require Import Coqlib Maps Integers Floats Values AST Errors.
+Require Import Globalenvs.
+Require Import Asm RelocProg RelocProgram.
+Require Import Hex compcert.encode.Bits Memdata Encode.
+Require Import BPProperty.
+Require Import TranslateInstr.
+Import Hex Bits.
+Import ListNotations.
+
+Local Open Scope error_monad_scope.
+Local Open Scope hex_scope.
+Local Open Scope bits_scope.
+
+Definition decode_instr l :=
+  match l with
+  | i :: l' =>
+      do i' <- decode_instr' i;
+      OK (i', l')
+  | _ => Error (msg "impossible")
+  end.
+
+Theorem translate_instr_consistency_aux: forall i i',
+    translate_instr' i = OK i' ->
+    decode_instr' i' = OK i.
+Proof.
+Admitted.
+
+Theorem translate_instr_consistency: forall i li l,
+    translate_instr i = OK li ->
+    decode_instr (li++l) = OK (i,l).
+Proof.
+  unfold translate_instr,decode_instr.
+  intros. monadInv H. simpl.
+  erewrite translate_instr_consistency_aux;eauto. simpl. auto.
+Qed.
