riscV/RelocBingenproofArchi.v
@@ -1,0 +1,106 @@
+Require Import Coqlib Maps AST lib.Integers Values.
+Require Import Events lib.Floats Memory Smallstep.
+Require Import Asm RelocProg RelocProgramBytes.
+Require Import Stacklayout Conventions.
+Require Import Linking RelocProgLinking Errors.   
+Require Import EncDecRet RelocBingen RelocBinDecode.
+Require Import RelocProgSemantics RelocProgSemantics1.
+Require Import TranslateInstr RelocProgSemantics2.
+Require Import RelocProgSemantics RelocProgSemantics1 RelocProgSemanticsArchi1.
+Require Import RelocProgSemanticsArchi RelocProgGlobalenvs.
+
+Import ListNotations.
+Local Open Scope error_monad_scope.
+
+
+Lemma encode_Instruction_not_empty:forall i,
+    encode_Instruction i = OK [] -> False.
+  destruct i;simpl; try (autounfold with bitfields;simpl;congruence;fail).
+  all: try (autounfold with bitfields;simpl;intros;repeat rewrite app_assoc in H;eapply app_cons_not_nil;inv H;eauto).
+Qed.
+
+Lemma translate_instr_not_empty : forall i,
+    translate_instr i = OK [] -> False.
+Proof.
+  destruct i;unfold translate_instr;simpl;intros;monadInv H.
+Qed.
+
+
+Section WITH_INSTR_SIZE.
+  Variable instr_size: instruction -> Z.
+
+
+Section PRESERVATION. 
+(** Transformation *)
+  Variable prog: RelocProgram.program.
+  Variable tprog: program.
+  
+  
+  Let ge := RelocProgSemantics1.globalenv instr_size prog.
+  Let tge := RelocProgSemantics2.globalenv instr_size tprog.
+  
+  Hypothesis symbol_address_pres: forall id ofs,
+    RelocProgGlobalenvs.Genv.symbol_address ge id ofs =
+    RelocProgGlobalenvs.Genv.symbol_address tge id ofs.
+  Hypothesis find_instr_refl: forall b ofs i,
+    Genv.genv_instrs ge b ofs = Some i ->
+    Genv.genv_instrs tge b ofs = Some i.
+  Hypothesis find_ext_funct_refl: forall v,
+    Genv.find_ext_funct ge v = Genv.find_ext_funct tge v.
+
+
+  Hypothesis senv_refl:
+    (Genv.genv_senv ge) = (Genv.genv_senv tge).
+
+
+Lemma step_simulation: forall st1 st2 t,
+    step instr_size ge st1 t st2 ->
+    step instr_size tge st1 t st2.
+Proof.
+  intros st1 st2 t STEP.
+  inv STEP.
+  - unfold Genv.find_instr in H1.
+    exploit find_instr_refl;eauto.
+    intros.
+    eapply exec_step_internal;eauto.
+    erewrite <- find_ext_funct_refl;eauto.
+    erewrite <- exec_instr_refl;eauto.
+
+  - 
+    rewrite find_ext_funct_refl in H0.
+    eapply exec_step_external;eauto.
+    rewrite <- senv_refl. auto.    
+Qed.
+
+Lemma initial_state_gen_match: forall rs m st tprog' (MAIN: prog_main prog = prog_main tprog),
+    decode_prog_code_section tprog = OK tprog' ->
+  initial_state_gen instr_size (decode_program instr_size prog) rs m st ->
+  exists st', initial_state_gen instr_size (decode_program instr_size tprog') rs m st' /\ st = st'.
+Proof.
+  intros.
+  inv H0.
+
+  set (ge2:= (globalenv instr_size (decode_program instr_size tprog'))).
+  set (rs0':= (((Pregmap.init Vundef) # PC <-
+           (Genv.symbol_address ge2 (prog_main (decode_program instr_size tprog')) Ptrofs.zero))
+                 # X2 <- Vnullptr) # X1 <- Vnullptr).
+  
+  exists (State rs0' m).
+  split.
+  econstructor;eauto.
+  f_equal. unfold rs0,rs0'.
+  generalize  symbol_address_pres.
+  unfold ge,tge. unfold RelocProgSemantics1.globalenv,RelocProgSemantics2.globalenv.
+  rewrite H. intros SYMB.
+  unfold ge0,ge2.
+  assert ((prog_main (decode_program instr_size prog)) = (prog_main (decode_program instr_size tprog'))).
+  unfold decode_program. unfold decode_prog_code_section in H.
+  monadInv H. simpl.  auto.
+
+  rewrite H0.
+  erewrite SYMB. auto.
+Qed.
+
+End PRESERVATION.
+
+End WITH_INSTR_SIZE.
